test/TestClause.v
@@ -5,7 +5,8 @@ Definition admin_all_clause :=
   {| cl_name := "admin_all"%bs;
      cl_head := PApp "allowed"%bs [PAtom "admin"%bs; PVar 0];
      cl_body := [];
-     cl_witness_args := [PVar 0] |}.
+     cl_witness_args := [PVar 0];
+     cl_npremises := None |}.
 
 Example admin_clause_name :
   cl_name admin_all_clause = "admin_all"%bs := eq_refl.
